Clean-up and restructering

src/HOL/CVC/cvc5_dsl_rewrites/Dsl_Nary_Ops.thy
@@ -18,29 +18,25 @@ additional assumption should be added to the lemma making sure that not all oper
 at the same time and a lemma should be proven below with the same assumption.
 
 *)
-(*TODO: QUESTION: Now that we don't always have neutral operators should this be replaced by SMTLIB
-neutrals that are just defined?*)
-named_theorems cvc_ListOp_neutral \<open>Neutral elements for cvc_ListOps\<close>
-lemma cvc_ListOp_neutral_and [cvc_ListOp_neutral]: "cvc_isListOp (ListOp (\<and>) True)" by simp
-lemma cvc_ListOp_neutral_or [cvc_ListOp_neutral]: "cvc_isListOp (ListOp (\<or>) False)" by simp
-lemma cvc_ListOp_neutral_plus [cvc_ListOp_neutral]: "cvc_isListOp (ListOp (+) (0::'a::monoid_add))" by simp
-lemma cvc_ListOp_neutral_plus_int [cvc_ListOp_neutral]: "cvc_isListOp (ListOp (+) (0::int))" by simp
-lemma cvc_ListOp_neutral_mult [cvc_ListOp_neutral]: "cvc_isListOp (ListOp (*) (1::int))" by simp
-lemma cvc_ListOp_neutral_append [cvc_ListOp_neutral]: "cvc_isListOp (ListOp (@) [])" by simp
-lemma cvc_ListOp_neutral_re_concat [cvc_ListOp_neutral]: "cvc_isListOp (ListOp (smtlib_re_concat) {''''})" 
-  by (simp add: smtlib_re_concat_def)
-lemma cvc_ListOp_neutral_str_concat [cvc_ListOp_neutral]: "cvc_isListOp (ListOp (smtlib_str_concat) [])"
-  by (simp add: smtlib_str_concat_def)
-lemma cvc_ListOp_neutral_re_union [cvc_ListOp_neutral]: "cvc_isListOp (ListOp (smtlib_re_union) {})"
-  by (simp add: smtlib_re_union_def)
-lemma cvc_ListOp_neutral_re_inter [cvc_ListOp_neutral]: "cvc_isListOp (ListOp (smtlib_re_inter) (UNIV))"
-  unfolding smtlib_re_inter_def by simp
-lemma cvc_ListOp_neutral_bv_xor [cvc_ListOp_neutral]: "cvc_isListOp (ListOp (semiring_bit_operations_class.xor) 0)"
-  by simp
-lemma cvc_ListOp_neutral_bv_or [cvc_ListOp_neutral]: "cvc_isListOp (ListOp (semiring_bit_operations_class.or) 0)"
-  by simp  
 
+lemma cvc_ListOp_neutral:
+  shows cvc_ListOp_neutral_and: "cvc_isListOp (ListOp (\<and>) True)"
+  and cvc_ListOp_neutral_or: "cvc_isListOp (ListOp (\<or>) False)"
+  and cvc_ListOp_neutral_plus: "cvc_isListOp (ListOp (+) (0::'a::monoid_add))"
+  and cvc_ListOp_neutral_plus_int: "cvc_isListOp (ListOp (+) (0::int))"
+  and cvc_ListOp_neutral_mult: "cvc_isListOp (ListOp (*) (1::int))"
+  and cvc_ListOp_neutral_append: "cvc_isListOp (ListOp (@) [])"
+  and cvc_ListOp_neutral_re_concat: "cvc_isListOp (ListOp (smtlib_re_concat) {''''})"
+  and cvc_ListOp_neutral_str_concat: "cvc_isListOp (ListOp (smtlib_str_concat) [])"
+  and cvc_ListOp_neutral_re_union: "cvc_isListOp (ListOp (smtlib_re_union) {})"
+  and cvc_ListOp_neutral_re_inter: "cvc_isListOp (ListOp (smtlib_re_inter) (UNIV))"
+  and cvc_ListOp_neutral_bv_xor: "cvc_isListOp (ListOp (semiring_bit_operations_class.xor) 0)"
+  and cvc_ListOp_neutral_bv_or: "cvc_isListOp (ListOp (semiring_bit_operations_class.or) 0)"
+  by (simp_all add: smtlib_re_concat_def smtlib_str_concat_def smtlib_re_union_def
+                    smtlib_re_inter_def)
 
+(*Since the SMT-LIB term parser in Isabelle parses all operators as right-associative we assume
+that this is the case. Further testing is needed to see if this is enough. *)
 
 fun cvc_nary_op_fold :: "('a \<Rightarrow> 'a \<Rightarrow> 'a) \<Rightarrow> 'a list \<Rightarrow> 'a" where
  cvc_nary_op_fold_Nil: "cvc_nary_op_fold op [x] = x" |
@@ -50,238 +46,193 @@ fun cvc_bin_op_fold :: "('a \<Rightarrow> 'a \<Rightarrow> 'a) \<Rightarrow> 'a 
  cvc_bin_op_fold_Nil: "cvc_bin_op_fold op [] y = y" |
  cvc_bin_op_fold_Cons: "cvc_bin_op_fold op (x#xs) y = (op x (cvc_bin_op_fold op xs y))"
 
-(*op xs a    (op x1 (op ... (op xn a)))*)
-(*and [] a = a *)
-(*and [x] a = and x a*)
+fun cvc_bin_op where
+ "cvc_bin_op op (ListVar xs) y = cvc_bin_op_fold op xs y"
+fun cvc_bin_op2 where
+ "cvc_bin_op2 op y (ListVar xs) = (if xs = [] then y else op y (cvc_nary_op_fold op xs))"
+fun cvc_bin_op3 where
+  "cvc_bin_op3 op (ListVar []) (ListVar []) neutral = neutral" | 
+  "cvc_bin_op3 op (ListVar xs) (ListVar []) neutral = cvc_nary_op_fold op xs" | 
+  "cvc_bin_op3 op (ListVar xs) (ListVar ys) neutral = cvc_bin_op_fold op xs (cvc_nary_op_fold op ys)"
 
-(*xs = [x1,xs], ys = [y1], zs = [(and z1 z2)]
-
-  "((cvc_list_left (\<and>) xs
- (cvc_list_right (\<and>) (cvc_list_right (\<and>) b ys) zs)) = (cvc_list_left (\<and>) xs
- (cvc_list_left (\<and>) zs (cvc_list_right (\<and>) b ys))))"
-
-xs = [x1, x2], ys = [y1], zs = [(and z1 z2)]
-
-(and x1 (and x2 (and (and b y1) (and z2 z3)))) = (and x1 (and x2 (and (and z1 z2) (and b y1)))
-
-
-
-(and x1 x2 (and b y1) (and z1 z2))
-
-*)
-fun cvc_bin_op where "cvc_bin_op op (ListVar xs) y = cvc_bin_op_fold op xs y"
-fun cvc_bin_op2 where "cvc_bin_op2 op y (ListVar xs) = (if xs = [] then y else op y (cvc_nary_op_fold op xs))"
-fun cvc_bin_op3 where "cvc_bin_op3 op (ListVar xs) (ListVar ys) neutral
-   = (if ys = [] \<and> xs = [] then neutral
-      else if ys = [] then (cvc_nary_op_fold op xs)
-      else cvc_bin_op_fold op xs (cvc_nary_op_fold op ys))"
-
-(* (\<and> b (\<or> xs ys))  = (\<and> b False) *)
-(* (\<or> b (\<or> xs ys))  =  b *)
 definition cvc_list_left where "cvc_list_left op lv y = cvc_bin_op op lv y"
 definition cvc_list_right where "cvc_list_right op y lv = cvc_bin_op2 op y lv"
 definition cvc_list_both where "cvc_list_both op neutral lv1 lv2 = cvc_bin_op3 op lv1 lv2 neutral"
 
-value "((cvc_list_left (\<and>) (ListVar [x1, x2])
- (cvc_list_right (\<and>) (cvc_list_right (\<and>) b (ListVar [y1])) (ListVar [(z1 \<and> z2)]))) = (cvc_list_left (\<and>) (ListVar [x1, x2])
- (cvc_list_left (\<and>) (ListVar [(z1 \<and> z2)]) (cvc_list_right (\<and>) b (ListVar [y1])))))"
-
-
-lemma transfer_h1:
+lemma cvc_nary_op_fold_transfer_h1:
   assumes "1 \<le> n" "cvc_isListOp (ListOp op neutral)"
-  shows "n = length xs \<longrightarrow> cvc_nary_op_fold op xs = foldr op xs neutral"
-proof-
-  have
-  "\<forall>xs. n = length xs \<longrightarrow> cvc_nary_op_fold op xs = foldr op xs neutral"
-    apply (rule nat_induct_at_least[of 1 n "\<lambda>n. \<forall>xs. n = length xs \<longrightarrow> cvc_nary_op_fold op xs = foldr op xs neutral"])
-    subgoal
-      using assms by simp
-    subgoal
-      proof(rule allI,rule impI)
-        fix xs::"'a list"
-        assume a0: "1 = length xs"
-        obtain x where t0: "[x] = xs"
-          by (metis One_nat_def Suc_length_conv a0 length_0_conv)
-        have "cvc_nary_op_fold op xs = x"
-          using t0 cvc_nary_op_fold_Nil by force
-        moreover have "foldr op xs neutral = (op x neutral)"
-          using t0 by force
-        ultimately show "cvc_nary_op_fold op xs = foldr op xs neutral"
-          using assms(2) by auto
-      qed
-      subgoal for n
-      proof(rule allI, rule impI)
-        fix xs::"'a list"
-        assume a0: "1 \<le> n"
-        assume a1: "\<forall>xs. n = length xs \<longrightarrow> cvc_nary_op_fold op xs = foldr op xs neutral"
-        assume a2: "Suc n = length xs"
-        then obtain x xss where t0: "xs = x#xss"
-          by (meson Suc_length_conv)
-        show "cvc_nary_op_fold op xs = foldr op xs neutral"
-        proof(cases "xss = []")
-          assume a00: "xss = []"
-          then have "cvc_nary_op_fold op xs = x" using t0 by auto
-          then show "cvc_nary_op_fold op xs = foldr op xs neutral"
-            using a0 a00 a2 t0 by auto
-        next
-          assume a01: "xss \<noteq> []"
-          then have "cvc_nary_op_fold op xs = op x (cvc_nary_op_fold op xss)" 
-            using cvc_nary_op_fold.elims(1) t0
-            by (metis list.inject list.simps(3))
-          then have "cvc_nary_op_fold op xs = op x (foldr op xss neutral)" 
-            using a1 a2 t0 by fastforce
-          then show "cvc_nary_op_fold op xs = (foldr op xs neutral)" 
-            by (simp add: t0)
-        qed
-      qed
-      done
-  then show ?thesis
-    by auto
-qed
-
+  shows "\<forall>xs. n = length xs \<longrightarrow> cvc_nary_op_fold op xs = foldr op xs neutral"
+  apply (induct_tac rule: nat_induct_at_least[of 1])
+  subgoal
+    using assms(1) by simp
+  subgoal
+    proof(rule allI,rule impI)
+    fix xs::"'a list"
+    assume a0: "1 = length xs"
+    obtain x where t0: "[x] = xs"
+      by (metis One_nat_def Suc_length_conv a0 length_0_conv)
+    have "cvc_nary_op_fold op xs = x"
+      using t0 cvc_nary_op_fold_Nil by force
+    moreover have "foldr op xs neutral = (op x neutral)"
+      using t0 by force
+    ultimately show "cvc_nary_op_fold op xs = foldr op xs neutral"
+      using assms(2) by auto
+  qed      
+  subgoal for n
+  proof(rule allI, rule impI)
+    fix xs::"'a list"
+    assume a0: "1 \<le> n"
+    assume a1: "\<forall>xs. n = length xs \<longrightarrow> cvc_nary_op_fold op xs = foldr op xs neutral"
+    assume a2: "Suc n = length xs"
+    then obtain x xss where t0: "xs = x#xss"
+      by (meson Suc_length_conv)
+    show "cvc_nary_op_fold op xs = foldr op xs neutral"
+    proof(cases "xss = []")
+      assume a00: "xss = []"
+      then show "cvc_nary_op_fold op xs = foldr op xs neutral"
+        using a0 a00 a2 t0 by auto
+    next
+      assume a01: "xss \<noteq> []"
+      then have "cvc_nary_op_fold op xs = op x (cvc_nary_op_fold op xss)" 
+        using cvc_nary_op_fold.elims(1) t0
+        by (metis list.inject list.simps(3))
+      then have "cvc_nary_op_fold op xs = op x (foldr op xss neutral)" 
+        using a1 a2 t0 by fastforce
+      then show "cvc_nary_op_fold op xs = (foldr op xs neutral)" 
+        by (simp add: t0)
+    qed
+  qed
+done
+  
 lemma cvc_nary_op_fold_transfer:
   assumes "1 \<le> length xs " "cvc_isListOp (ListOp op neutral)"
   shows "cvc_nary_op_fold op xs = foldr op xs neutral"
-  using transfer_h1 assms by metis
+  by (meson assms(1) assms(2) cvc_nary_op_fold_transfer_h1)
 
-lemma cvc_bin_op_fold_transfer:
-  shows "cvc_bin_op_fold op xs y = foldr op xs y"
+lemma cvc_bin_op_fold_transfer: "cvc_bin_op_fold op xs y = foldr op xs y"
   apply (induction xs)
   by auto
+
+(*Left Transfer*)
 
 lemma cvc_list_left_transfer:
   shows "cvc_list_left op (ListVar xs) y = foldr op xs y"
   by (simp add: cvc_list_left_def cvc_bin_op_fold_transfer)
 
-lemma cvc_list_right_transfer2': 
-  assumes "cvc_isListOp (ListOp op neutral)"
-  shows "cvc_list_right op y (ListVar xs) = (foldr op (y#xs) neutral)"
-  apply (cases xs)
-  unfolding cvc_list_right_def
-  using assms apply auto[1]
-  by (metis Dsl_Nary_Ops.cvc_nary_op_fold_Cons One_nat_def assms cvc_bin_op2.simps le_numeral_extra(4) list.distinct(1) list.size(4) trans_le_add2 transfer_h1)
+(*Right Transfer*)
 
-
-lemma cvc_list_right_transfer: 
+lemma cvc_list_right_transfer_neutral1: 
   assumes "cvc_isListOp (ListOp op neutral)"
   shows "cvc_list_right op y (ListVar xs) = op y (foldr op xs neutral)"
+  using assms
+  unfolding cvc_list_right_def
   apply (cases xs)
-   apply simp
-  using assms cvc_list_right_def
-  apply (metis cvc_bin_op2.simps cvc_isListOp.simps)
-  using assms cvc_list_right_def cvc_nary_op_fold_transfer
-  by (metis One_nat_def cvc_bin_op2.simps le_numeral_extra(4) list.simps(3) list.size(4) trans_le_add2)
+  by (simp_all add: cvc_nary_op_fold_transfer)
 
-(*TODO: clean-up*)
-lemma cvc_list_right_transfer_h1:
-"cvc_list_right op y (ListVar (xs @ [xn])) = op y (foldr op xs xn)"
+lemma cvc_list_right_transfer_neutral2: 
+  assumes "cvc_isListOp (ListOp op neutral)"
+  shows "cvc_list_right op y (ListVar xs) = (foldr op (y#xs) neutral)"
+  using assms
+  unfolding cvc_list_right_def
+  apply (cases xs)
+  by (simp_all add: cvc_nary_op_fold_transfer)
+
+lemma cvc_list_right_transfer:
+  "cvc_list_right op y (ListVar (xs @ [xn])) = op y (foldr op xs xn)"
   apply (induction xs arbitrary: y)
-   apply simp_all
-   apply (simp add: cvc_list_right_def)
   unfolding cvc_list_right_def
   apply simp
-  subgoal for x1 xss y
+  subgoal for x1 xss yshows
     apply (cases xss)
     by simp_all
   done
 
-
-lemma cvc_list_right_transfer3: 
+lemma cvc_list_right_transfer_2: 
   assumes "xs \<noteq> []"
   shows "cvc_list_right op y (ListVar xs) = (foldr op (y # butlast xs) (last xs))"
   apply (cases "rev xs")
   using assms apply force
-  using cvc_list_right_transfer_h1
-  by (metis Dsl_Nary_Ops.cvc_bin_op_fold_Cons butlast_snoc cvc_bin_op_fold_transfer last_snoc rev_eq_Cons_iff)
+  by (simp add: cvc_list_right_transfer)
 
-
-lemma cvc_list_right_transfer2: 
-  assumes "xs \<noteq> []"
-  shows "cvc_list_right op y (ListVar xs) = op y (foldr op (butlast xs) (last xs))"
-  apply (cases "rev xs")
-  using assms apply force
-  using cvc_list_right_transfer_h1
-  by (metis Nil_is_rev_conv append_butlast_last_id list.distinct(1))
-
-
+(*TODO: Hopefully these can be safely deleted after testing is complete*)
 named_theorems cvc_list_right_transfer_op \<open>cvc_list_right_transfer instantiated with operator\<close>
 
 lemma [cvc_list_right_transfer_op]: 
   "cvc_list_right (\<and>) y (ListVar xs) = (\<and>) y (foldr (\<and>) xs True)"
-  by (simp add: cvc_list_right_transfer)
+  by (simp add: cvc_list_right_transfer_neutral1)
 
 lemma [cvc_list_right_transfer_op]:
   "cvc_list_right (\<or>) y (ListVar xs) = (\<or>) y (foldr (\<or>) xs False)"
-  by (simp add: cvc_list_right_transfer)
+  by (simp add: cvc_list_right_transfer_neutral1)
 
 lemma [cvc_list_right_transfer_op]:
   "cvc_list_right (+) y (ListVar xs) = (+) y (foldr (+) xs (0::int))"
-  by (simp add: cvc_list_right_transfer)
+  by (simp add: cvc_list_right_transfer_neutral1)
 
 lemma [cvc_list_right_transfer_op]:
   "cvc_list_right (+) y (ListVar xs) = (+) y (foldr (+) xs (0::'a::monoid_add))"
-  by (simp add: cvc_list_right_transfer)
+  by (simp add: cvc_list_right_transfer_neutral1)
 
 lemma [cvc_list_right_transfer_op]:
   "cvc_list_right (*) y (ListVar xs) = (*) y (foldr (*) xs (1::int))"
-  by (simp add: cvc_list_right_transfer)
+  by (simp add: cvc_list_right_transfer_neutral1)
 
 lemma [cvc_list_right_transfer_op]:
   "cvc_list_right (*) y (ListVar xs) = (*) y (foldr (*) xs (1::'a::monoid_mult))"
-  by (simp add: cvc_list_right_transfer)
+  by (simp add: cvc_list_right_transfer_neutral1)
 
 lemma [cvc_list_right_transfer_op]:
   "cvc_list_right (@) y (ListVar xs) = (@) y (foldr (@) xs [])"
-  by (simp add: cvc_list_right_transfer)
+  by (simp add: cvc_list_right_transfer_neutral1)
 
 lemma [cvc_list_right_transfer_op]:
-  "cvc_list_right (smtlib_re_concat) y (ListVar xs) = (smtlib_re_concat) y (foldr (smtlib_re_concat) xs {''''})"
-  by (meson cvc_ListOp_neutral_re_concat cvc_list_right_transfer)
+  "cvc_list_right (smtlib_re_concat) y (ListVar xs)
+   = (smtlib_re_concat) y (foldr (smtlib_re_concat) xs {''''})"
+  by (meson cvc_ListOp_neutral_re_concat cvc_list_right_transfer_neutral1)
 
 lemma [cvc_list_right_transfer_op]:
-  "cvc_list_right (smtlib_str_concat) y (ListVar xs) = (smtlib_str_concat) y (foldr (smtlib_str_concat) xs [])"
-  by (simp add: cvc_list_right_transfer smtlib_str_concat_def)
+  "cvc_list_right (smtlib_str_concat) y (ListVar xs)
+   = (smtlib_str_concat) y (foldr (smtlib_str_concat) xs [])"
+  by (simp add: cvc_list_right_transfer_neutral1 smtlib_str_concat_def)
 
 lemma [cvc_list_right_transfer_op]:
-  "cvc_list_right (smtlib_re_union) y (ListVar xs) = (smtlib_re_union) y (foldr (smtlib_re_union) xs {})"
-  by (meson cvc_ListOp_neutral_re_union cvc_list_right_transfer)
+  "cvc_list_right (smtlib_re_union) y (ListVar xs)
+   = (smtlib_re_union) y (foldr (smtlib_re_union) xs {})"
+  by (meson cvc_ListOp_neutral_re_union cvc_list_right_transfer_neutral1)
 
 lemma [cvc_list_right_transfer_op]:
-  "cvc_list_right (smtlib_re_inter) y (ListVar xs) = (smtlib_re_inter) y (foldr (smtlib_re_inter) xs (UNIV))"
-  by (meson cvc_ListOp_neutral_re_inter cvc_list_right_transfer)
+  "cvc_list_right (smtlib_re_inter) y (ListVar xs)
+   = (smtlib_re_inter) y (foldr (smtlib_re_inter) xs (UNIV))"
+  by (meson cvc_ListOp_neutral_re_inter cvc_list_right_transfer_neutral1)
 
 lemma [cvc_list_right_transfer_op]:
-  "cvc_list_right (semiring_bit_operations_class.xor) y (ListVar xs) = (semiring_bit_operations_class.xor) y (foldr (semiring_bit_operations_class.xor) xs 0)"
-  by (simp add: cvc_list_right_transfer smtlib_str_concat_def)
+  "cvc_list_right (semiring_bit_operations_class.xor) y (ListVar xs)
+   = (semiring_bit_operations_class.xor) y (foldr (semiring_bit_operations_class.xor) xs 0)"
+  by (simp add: cvc_list_right_transfer_neutral1)
 
 lemma [cvc_list_right_transfer_op]:
-  "cvc_list_right (semiring_bit_operations_class.or) y (ListVar xs) = (semiring_bit_operations_class.or) y (foldr (semiring_bit_operations_class.or) xs 0)"
-  by (simp add: cvc_list_right_transfer smtlib_str_concat_def)
+  "cvc_list_right (semiring_bit_operations_class.or) y (ListVar xs)
+   = (semiring_bit_operations_class.or) y (foldr (semiring_bit_operations_class.or) xs 0)"
+  by (simp add: cvc_list_right_transfer_neutral1)
 
 lemma [cvc_list_right_transfer_op]:
-  "xs \<noteq> [] \<longrightarrow> cvc_list_right (semiring_bit_operations_class.and) y (ListVar xs) = (semiring_bit_operations_class.and) y (foldr (semiring_bit_operations_class.and) (butlast xs) (last xs))"
-  using cvc_list_right_transfer2[of xs "(semiring_bit_operations_class.and)" y]
-  by blast
+  "xs \<noteq> [] \<longrightarrow> cvc_list_right (semiring_bit_operations_class.and) y (ListVar xs)
+   = (semiring_bit_operations_class.and) y (foldr (semiring_bit_operations_class.and) (butlast xs)
+   (last xs))"
+  by (simp add: cvc_list_right_transfer_2)
 
 
-
+(*Both Transfer*)
 
 lemma cvc_list_both_transfer: 
   assumes "cvc_isListOp (ListOp op neutral)"
   shows "cvc_list_both op neutral (ListVar ys) (ListVar xs) = foldr op ys (foldr op xs neutral)"
   using assms
-  apply (cases "xs = [] \<and> ys = []")
-   apply simp
   unfolding cvc_list_both_def
-  apply simp
-  apply (cases ys)
-  unfolding cvc_list_both_def
-    apply simp
-  apply (metis assms(1) cvc_bin_op2.simps cvc_list_right_def cvc_list_right_transfer)
-  by (metis One_nat_def cvc_bin_op.simps cvc_bin_op3.simps cvc_bin_op_fold_transfer cvc_nary_op_fold_transfer foldr.simps(1) id_apply length_0_conv less_Suc0 linorder_not_less)
+  apply(cases \<open>(op,(ListVar ys),(ListVar xs),neutral)\<close>  rule: cvc_bin_op3.cases)
+  by (simp_all add: cvc_bin_op_fold_transfer cvc_nary_op_fold_transfer)
 
 named_theorems cvc_list_both_transfer_op \<open>cvc_list_both_transfer instantiated with operator\<close>
-
 
 lemma [cvc_list_both_transfer_op]: 
   "cvc_list_both (\<and>) True (ListVar ys) (ListVar xs) = foldr (\<and>) ys (foldr (\<and>) xs True)"
